Atomics.thy
@@ -15,20 +15,6 @@ text \<open>Weakest precondition of a basic instruction, based on the locale's
 abbreviation wp\<^sub>\<alpha> :: "('a,'b) basic \<Rightarrow> 'b pred \<Rightarrow> 'b pred"
   where "wp\<^sub>\<alpha> \<alpha> Q \<equiv> wp (vc \<alpha>) (beh \<alpha>) Q"
 
-(*
-text \<open>Weakest precondition of a program, only covering basic instructions, environment steps and 
-      sequential composition as these are sufficient for the logic's checks.\<close>
-fun wp\<^sub>c :: "('a,'b) com \<Rightarrow> 'b pred \<Rightarrow> 'b pred"
-  where 
-    "wp\<^sub>c (Basic \<alpha>) Q = wp\<^sub>\<alpha> \<alpha> Q" |
-    "wp\<^sub>c (Seq c\<^sub>1 c\<^sub>2) Q = wp\<^sub>c c\<^sub>1 (wp\<^sub>c c\<^sub>2 Q)" |
-    "wp\<^sub>c _ Q = undefined"
-
-text \<open>Refinement relation between two programs, in terms of their weakest precondition calculation.\<close>
-definition refine :: "('a,'b) com \<Rightarrow> ('a,'b) com \<Rightarrow> bool" (infix "\<sqsubseteq>" 60)
-  where "c \<sqsubseteq> c' \<equiv> \<forall>Q. wp\<^sub>c c Q \<subseteq> wp\<^sub>c c' Q"
-*)
-
 text \<open>Specification check, ensuring an instruction conforms to a relation\<close>
 abbreviation guar\<^sub>\<alpha> :: "('a,'b) basic \<Rightarrow> 'b rpred \<Rightarrow> bool"
   where "guar\<^sub>\<alpha> \<alpha> G \<equiv> guar (vc \<alpha>) (beh \<alpha>) G"
