Rules.thy
@@ -20,7 +20,9 @@ inductive rules :: "'b rpred \<Rightarrow> 'b rpred \<Rightarrow> 'b set \<Right
   basic[intro]:  "R,G \<turnstile>\<^sub>A P {\<alpha>} Q \<Longrightarrow> R,G \<turnstile> P { Basic \<alpha> } Q" |
   nil[intro]:    "stable R P \<Longrightarrow> R,G \<turnstile> P { Nil } P" |
   seq[intro]:    "R,G \<turnstile> Q { c\<^sub>2 } M \<Longrightarrow> R,G \<turnstile> P { c\<^sub>1 } Q \<Longrightarrow> R,G \<turnstile> P { c\<^sub>1 ;; c\<^sub>2 } M" |
+  ord[intro]:    "R,G \<turnstile> Q { c\<^sub>2 } M \<Longrightarrow> R,G \<turnstile> P { c\<^sub>1 } Q \<Longrightarrow> R,G \<turnstile> P { c\<^sub>1 \<cdot> c\<^sub>2 } M" |
   choice[intro]: "R,G \<turnstile> P { c\<^sub>1 } Q \<Longrightarrow> R,G \<turnstile> P { c\<^sub>2 } Q \<Longrightarrow> R,G \<turnstile> P { c\<^sub>1 \<sqinter> c\<^sub>2 } Q" |
+  seqset[intro]: "\<forall>s \<in> S. R,G \<turnstile> P { seq2com s } Q \<Longrightarrow> R,G \<turnstile> P { \<Sqinter> S } Q" |
   loop[intro]:   "stable R P \<Longrightarrow> R,G \<turnstile> P { c } P \<Longrightarrow> R,G \<turnstile> P { c* } P" |
   thread[intro]: "R,G \<turnstile> P { c } Q \<Longrightarrow> rif R G c \<Longrightarrow> R,G \<turnstile> P { Thread c } Q" |
   par[intro]:    "R\<^sub>1,G\<^sub>1 \<turnstile> P\<^sub>1 { c\<^sub>1 } Q\<^sub>1 \<Longrightarrow> R\<^sub>2,G\<^sub>2 \<turnstile> P\<^sub>2 { c\<^sub>2 } Q\<^sub>2 \<Longrightarrow> G\<^sub>2 \<subseteq> R\<^sub>1 \<Longrightarrow> G\<^sub>1 \<subseteq> R\<^sub>2 \<Longrightarrow> 
@@ -61,6 +63,11 @@ lemma seqE [elim]:
   obtains M  where "R,G \<turnstile> P {c\<^sub>1} M" "R,G \<turnstile> M {c\<^sub>2} Q"
   using assms by (induct R G P "c\<^sub>1 ;; c\<^sub>2" Q arbitrary: c\<^sub>1 c\<^sub>2) blast+ 
 
+lemma ordE [elim]:
+  assumes "R,G \<turnstile> P {c\<^sub>1 \<cdot> c\<^sub>2} Q"
+  obtains M  where "R,G \<turnstile> P {c\<^sub>1} M" "R,G \<turnstile> M {c\<^sub>2} Q"
+  using assms by (induct R G P "c\<^sub>1 \<cdot> c\<^sub>2" Q arbitrary: c\<^sub>1 c\<^sub>2) blast+
+
 text \<open>It is always possible to rephrase a judgement in terms of a stable precondition\<close>
 lemma stable_preE:
   assumes "R,G \<turnstile> P {c} Q"
@@ -91,13 +98,29 @@ next
   case (inv R G P c Q R' I)
   then obtain P' where "P \<subseteq> P'" "stable R P'" "R,G \<turnstile> P' {c} Q" by auto
   then show ?case using inv rules.inv by blast
+next
+  case (seqset S R G P Q)
+  hence "\<exists>P\<^sub>s. \<forall>s\<in>S. P \<subseteq> P\<^sub>s s \<and> stable R (P\<^sub>s s) \<and> (R,G \<turnstile> P\<^sub>s s {seq2com s} Q)"
+    by metis
+  then obtain P\<^sub>s where s: "\<forall>s\<in>S. P \<subseteq> P\<^sub>s s \<and> stable R (P\<^sub>s s) \<and> (R,G \<turnstile> P\<^sub>s s {seq2com s} Q)"
+    by blast
+  hence "stable R (\<Inter>s\<in>S. P\<^sub>s s)" by (auto simp: stable_def)
+  moreover have "P \<subseteq> (\<Inter>s\<in>S. P\<^sub>s s)" using s by auto
+  ultimately show ?case using s seqset.hyps(1) by blast
 qed blast+
+
+lemma false_seqI [intro]:
+  "\<forall>\<beta> \<in> set s. guar\<^sub>\<alpha> \<beta> G \<Longrightarrow> R,G \<turnstile> {} {seq2com s} {}"
+  by (induct s) auto
 
 lemma falseI:
   "local c \<Longrightarrow> \<forall>\<beta> \<in> basics c. guar\<^sub>\<alpha> \<beta> G \<Longrightarrow> R,G \<turnstile> {} {c} {}"
 proof (induct c)
   case (Basic x)
-  thus ?case by (intro basic atomic_falseI) auto
+  thus ?case by (intro basic) (auto simp: atomic_rule_def guar_def wp_def)
+next
+  case (SeqChoice x)
+  thus ?case by (intro ballI seqset false_seqI) auto
 qed auto
 
 end
